Add concurrent/spmc_stack.spmc_stack_of_mpmc_stack and concurrent/spmc_queue.spmc_queue_of_mpmc_queue.

theories/concurrent/spmc_queue.v
@@ -1,7 +1,10 @@
 From caml5 Require Import
   prelude.
+From caml5.base_logic Require Import
+  lib.excl.
 From caml5.lang Require Import
-  notations.
+  notations
+  proofmode.
 From caml5.concurrent Require Export
   base.
 From caml5.concurrent Require Import
@@ -26,6 +29,11 @@ Record spmc_queue `{!heapGS Σ} := {
     Timeless (spmc_queue_model t γ vs) ;
   spmc_queue_producer_timeless t γ :
     Timeless (spmc_queue_producer t γ) ;
+
+  spmc_queue_producer_exclusive t γ :
+    spmc_queue_producer t γ -∗
+    spmc_queue_producer t γ -∗
+    False ;
 
   spmc_queue_make_spec ι :
     {{{ True }}}
@@ -64,31 +72,69 @@ Record spmc_queue `{!heapGS Σ} := {
     >>> ;
 }.
 #[global] Arguments spmc_queue _ {_} : assert.
-#[global] Arguments Build_spmc_queue {_ _ _ _ _ _ _ _ _ _ _ _} _ _ _ : assert.
+#[global] Arguments Build_spmc_queue {_ _ _ _ _ _ _ _ _ _ _ _ _} _ _ _ : assert.
 #[global] Existing Instance spmc_queue_inv_persistent.
 #[global] Existing Instance spmc_queue_model_timeless.
 #[global] Existing Instance spmc_queue_producer_timeless.
 
-Program Definition spmc_queue_of_mpmc_queue `{!heapGS Σ} mpmc_queue := {|
-  spmc_queue_make := mpmc_queue.(mpmc_queue_make) ;
-  spmc_queue_push := mpmc_queue.(mpmc_queue_push) ;
-  spmc_queue_pop := mpmc_queue.(mpmc_queue_pop) ;
+Class SpmcQueueOfMpmcQueueG Σ `{!heapGS Σ} := {
+  spmc_queue_of_mpmc_queue_G_producer_G : ExclG Σ unitO ;
+}.
+#[local] Existing Instance spmc_queue_of_mpmc_queue_G_producer_G.
 
-  spmc_queue_name := mpmc_queue.(mpmc_queue_name) ;
-  spmc_queue_inv := mpmc_queue.(mpmc_queue_inv) ;
-  spmc_queue_model := mpmc_queue.(mpmc_queue_model) ;
-  spmc_queue_producer _ _ := True%I ;
-|}.
-Next Obligation.
-  intros.
-  setoid_rewrite (@right_id _ equiv True%I); last apply _.
-  apply mpmc_queue_make_spec.
+Definition spmc_queue_of_mpmc_queue_Σ := #[
+  excl_Σ unitO
+].
+Lemma subG_spmc_queue_of_mpmc_queue_Σ Σ `{!heapGS Σ} :
+  subG spmc_queue_of_mpmc_queue_Σ Σ →
+  SpmcQueueOfMpmcQueueG Σ.
+Proof.
+  solve_inG.
 Qed.
-Next Obligation.
-  intros.
-  rewrite /atomic_triple. setoid_rewrite (@right_id _ equiv True%I); last apply _.
-  apply mpmc_queue_push_spec.
-Qed.
-Next Obligation.
-  intros. apply mpmc_queue_pop_spec.
-Qed.
+
+Section spmc_queue_of_mpmc_queue.
+  Context `{SpmcQueueOfMpmcQueueG Σ} (mpmc_queue : mpmc_queue Σ).
+
+  Notation "γ .(base)" := γ.1
+  ( at level 5
+  ) : stdpp_scope.
+  Notation "γ .(producer)" := γ.2
+  ( at level 5
+  ) : stdpp_scope.
+
+  Program Definition spmc_queue_of_mpmc_queue := {|
+    spmc_queue_make :=
+      mpmc_queue.(mpmc_queue_make) ;
+    spmc_queue_push :=
+      mpmc_queue.(mpmc_queue_push) ;
+    spmc_queue_pop :=
+      mpmc_queue.(mpmc_queue_pop) ;
+
+    spmc_queue_name :=
+      mpmc_queue.(mpmc_queue_name) * gname ;
+    spmc_queue_inv t γ ι :=
+      mpmc_queue.(mpmc_queue_inv) t γ.(base) ι ;
+    spmc_queue_model t γ :=
+      mpmc_queue.(mpmc_queue_model) t γ.(base) ;
+    spmc_queue_producer _ γ :=
+      excl γ.(producer) () ;
+  |}.
+  Next Obligation.
+    intros. apply excl_exclusive.
+  Qed.
+  Next Obligation.
+    iIntros "%ι %Φ _ HΦ".
+    iMod excl_alloc as "(%γ_producer & Hproducer)".
+    wp_apply (mpmc_queue_make_spec with "[//]"). iIntros "%t %γ_base (Hinv & Hmodel)".
+    iApply ("HΦ" $! t (γ_base, γ_producer)). iFrame.
+  Qed.
+  Next Obligation.
+    iIntros "%t %γ %ι %v !> %Φ (Hinv & Hproducer) HΦ".
+    wp_apply (mpmc_queue_push_spec with "Hinv").
+    iApply (atomic_update_wand with "[Hproducer] HΦ").
+    iIntros "_ HΦ _". iApply "HΦ". done.
+  Qed.
+  Next Obligation.
+    intros. apply mpmc_queue_pop_spec.
+  Qed.
+End spmc_queue_of_mpmc_queue.
